debug elpi context variables with ugly hacks :ambulance:

examples/examples.v
@@ -32,6 +32,13 @@ Local Open Scope Z_scope.
 Goal forall (l : list Z) (x : Z), hd_error l = Some x -> (l <> nil).
 Proof. snipe. Qed.
 
+Fixpoint zip {A B : Type} (l : list A) (l' : list B) :=
+  match l, l' with
+  | [], _ => []
+  | x :: xs, [] => []
+  | x :: xs, y :: ys => (x, y) :: zip xs ys 
+  end.
+
 
 (* The `snipe` tactics requires instances of equality to be decidable.
    It is in particular visible with type variables. *)
@@ -163,6 +170,71 @@ Lemma map_compound : forall (A B C : Type) (HA : CompDec A)
 map g (map f l) = map (fun x => g (f x)) l.
 Proof.
 induction l; snipe2. Qed.
+
+(* Section higher_order.
+
+Variable A : Type.
+Variable HA : CompDec A.
+Variable B : Type.
+Variable HB : CompDec B.*)
+From elpi Require Import elpi.
+
+Elpi Tactic elimination_polymorphism'.
+Elpi Accumulate File "elpi/utilities.elpi".
+Elpi Accumulate File "elpi/instantiate.elpi".
+Elpi Accumulate File "elpi/find_instances.elpi".
+Elpi Accumulate File "elpi/construct_cuts.elpi".
+
+Elpi Accumulate lp:{{
+
+ pred instances_param_indu_strategy_list i: list (pair term term), i: list (pair term (list instance)), i: goal, o: list sealed-goal.
+    instances_param_indu_strategy_list [P | XS] Inst (goal Ctx _ _ _ _ as G) GS :-
+      std.rev Ctx Ctx',
+      subst_in_instances Ctx' Inst Inst',
+      snd P HPoly,
+      instances_param_indu_strategy_aux HPoly Inst' [{{unit}}] LInst, !, coq.say "LINST" LInst,
+      % unit is a dumb default case to eliminate useless polymorphic premise
+      construct_cuts LInst ProofTerm,
+      refine ProofTerm G GL1, !,
+      refine_by_instantiation GL1 P [G1|_GL], !, 
+      coq.ltac.open (instances_param_indu_strategy_list XS Inst) G1 GS.
+    instances_param_indu_strategy_list [] _ _G _.
+    
+  solve (goal Ctx _ TyG _ L as G) GL :- std.rev Ctx Ctx',
+    collect_hypotheses_from_context Ctx HL HL1, polymorphic_hypotheses HL1 HL2, argument_to_term L LTerm, 
+    append_nodup HL2 LTerm HPoly, !, find_instantiated_params_in_list Ctx' [TyG |HL] Inst,
+    instances_param_indu_strategy_list HPoly Inst G GL.
+ 
+
+}}.
+Elpi Typecheck.
+
+Ltac clear_prenex_poly_hyps_in_context := repeat match goal with 
+| H : forall (A : ?T), _ |- _ => first [ constr_eq T Set | constr_eq T Type] ; 
+let T := type of H in let U := type of T in tryif (constr_eq U Prop) then try (clear H)
+else fail
+end.
+
+Tactic Notation "elimination_polymorphism" uconstr_list_sep(l, ",") :=
+  elpi elimination_polymorphism ltac_term_list:(l) ; clear_prenex_poly_hyps_in_context.
+
+Tactic Notation "scope2_aux" constr(p1) constr(p2) uconstr_list_sep(l, ",") := 
+let p2' := eval unfold p2 in p2 in
+intros ; 
+repeat match goal with
+| H : _ |- _  => eliminate_dependent_pattern_matching H
+| _ => fail
+end ;
+try interp_alg_types_context_goal p2' ; try (def_fix_and_pattern_matching p1 ltac:(get_definitions_theories_no_generalize)) ; 
+elpi elimination_polymorphism' ltac_term_list:(l) ; clear_prenex_poly_hyps_in_context ;
+get_projs_in_variables p2'.
+
+Lemma zip_map A B (f : A -> B) (g : A -> B) (l : list A) :
+map (fun (x : A) => (f x, g x)) l = zip (map f l) (map g l).
+Proof. (* The pb is that f and g are also context variables so should be substituted in hypothesis *)
+induction l ; scope2_aux prod_of_symb prod_types. Qed.
+
+End higher_order.
 
 (** Examples on trees *)
 
